Split out some files, use (better?) eval_app

extraction/theories/OptimizeCorrectness.v
@@ -1,6 +1,8 @@
+From ConCert.Extraction Require Import Aux.
 From ConCert.Extraction Require Import ExAst.
 From ConCert.Extraction Require Import ExTyping.
 From ConCert.Extraction Require Import Optimize.
+From ConCert.Extraction Require Import WcbvEvalAux.
 From Coq Require Import Arith.
 From Coq Require Import Bool.
 From Coq Require Import String.
@@ -20,29 +22,6 @@ Set Equations Transparent.
 Import EAstUtils.
 Import Erasure.
 Import ExAst.
-SearchAbout (negb _ = false).
-
-Ltac propize :=
-  unfold is_true in *;
-  repeat
-    match goal with
-    | [H: context[orb _ _ = false] |- _] => rewrite Bool.orb_false_iff in H
-    | [H: context[orb _ _ = true] |- _] => rewrite Bool.orb_true_iff in H
-    | [|- context[orb _ _ = false]] => rewrite Bool.orb_false_iff
-    | [|- context[orb _ _ = true]] => rewrite Bool.orb_true_iff
-    | [H: context[andb _ _ = false] |- _] => rewrite Bool.andb_false_iff in H
-    | [H: context[andb _ _ = true] |- _] => rewrite Bool.andb_true_iff in H
-    | [H: context[negb _ = true] |- _] => rewrite Bool.negb_true_iff in H
-    | [H: context[negb _ = false] |- _] => rewrite Bool.negb_false_iff in H
-    | [|- context[andb _ _ = false]] => rewrite Bool.andb_false_iff
-    | [|- context[andb _ _ = true]] => rewrite Bool.andb_true_iff
-    | [H: context[Nat.ltb _ _ = true] |- _] => rewrite Nat.ltb_lt in H
-    | [H: context[Nat.ltb _ _ = false] |- _] => rewrite Nat.ltb_ge in H
-    | [H: context[Nat.eqb _ _ = true] |- _] => rewrite Nat.eqb_eq in H
-    | [H: context[Nat.eqb _ _ = false] |- _] => rewrite Nat.eqb_neq in H
-    | [|- context[Nat.eqb _ _ = true]] => rewrite Nat.eqb_eq
-    | [|- context[Nat.eqb _ _ = false]] => rewrite Nat.eqb_neq
-    end.
 
 (* We have our own environment which is different from MetaCoq's erased environment
    (it includes more information and a different treatment of types).
@@ -76,8 +55,6 @@ Proof.
     + inversion lookup_decl; subst; easy.
     + auto.
 Qed.
-
-Local Notation "Σ ⊢ s ▷ t" := (eval Σ s t) (at level 50, s, t at next level) : type_scope.
 
 Lemma eval_only_constants Σ s t :
   Σ ⊢ s ▷ t ->
@@ -115,155 +92,6 @@ Proof.
     unfold eq_kername in lookup.
     now destruct (kername_eq_dec _ _).
 Qed.
-
-(*
-Section eta_correctness.
-Context (ctors : list (inductive * nat * nat)).
-Context (consts : list (kername * nat)).
-
-Notation eta_ctor := (eta_ctor ctors).
-Notation eta_const := (eta_const consts).
-Notation eta_expand_aux := (eta_expand_aux ctors consts).
-Notation eta_expand := (eta_expand ctors consts).
-
-Open Scope type.
-
-Lemma wfe_term_eta_single Σ t args n :
-  wfe_term Σ t ->
-  Forall (wfe_term Σ) args ->
-  wfe_term Σ (eta_single t args n).
-Proof.
-  intros wft wfall.
-  unfold eta_single.
-  induction (_ - _) at 3; [|easy].
-  cbn in *.
-  apply wfe_term_mkApps; [easy|].
-  apply Forall_app_inv.
-  - clear -wfall.
-    generalize args at 1; intros.
-    induction wfall; cbn in *; [easy|].
-    constructor; [|easy].
-    now apply wfe_term_lift.
-  - clear.
-    induction (seq _ _); [cbn; easy|].
-    rewrite rev_map_cons.
-    apply Forall_app_inv; [easy|].
-    constructor; easy.
-Qed.
-
-Lemma wfe_term_eta_ctor Σ ind i args :
-  wfe_term Σ (tConstruct ind i) ->
-  Forall (wfe_term Σ) args ->
-  wfe_term Σ (eta_ctor ind i args).
-Proof.
-  intros wft wfall.
-  unfold eta_ctor.
-  destruct (find _ _) as [((? & ?) & ?)|].
-  - now apply wfe_term_eta_single.
-  - now apply wfe_term_mkApps.
-Qed.
-
-Lemma wfe_term_eta_const Σ kn args :
-  wfe_term Σ (tConst kn) ->
-  Forall (wfe_term Σ) args ->
-  wfe_term Σ (eta_const kn args).
-Proof.
-  intros wft wfall.
-  unfold eta_const.
-  destruct (find _ _) as [((? & ?) & ?)|].
-  - now apply wfe_term_eta_single.
-  - now apply wfe_term_mkApps.
-Qed.
-
-Lemma wfe_term_eta_expand_aux Σ args t :
-  Forall (wfe_term Σ) args ->
-  wfe_term Σ t ->
-  wfe_term Σ (eta_expand_aux args t).
-Proof.
-  revert args.
-  induction t using term_forall_list_ind; intros args wfall wft; cbn in *; auto.
-  - now apply wfe_term_mkApps.
-  - now apply wfe_term_mkApps.
-  - now apply wfe_term_mkApps.
-  - apply wfe_term_mkApps; [|easy].
-    now induction H; cbn in *.
-  - now apply wfe_term_mkApps.
-  - apply wfe_term_mkApps; cbn; easy.
-  - apply IHt1; [|easy].
-    constructor; [|easy].
-    now apply IHt2.
-  - now apply wfe_term_eta_const.
-  - now apply wfe_term_eta_ctor.
-  - apply wfe_term_mkApps; [|easy].
-    cbn.
-    destruct p.
-    split; [easy|].
-    split; [easy|].
-    destruct wft as (_ & (_ & allwf)).
-    induction X; cbn in *; easy.
-  - now apply wfe_term_mkApps.
-  - apply wfe_term_mkApps; [|easy].
-    induction H; cbn in *; easy.
-  - apply wfe_term_mkApps; [|easy].
-    induction H; cbn in *; easy.
-Qed.
-
-Lemma wfe_term_eta_expand Σ t :
-  wfe_term Σ t ->
-  wfe_term Σ (eta_expand t).
-Proof. now apply wfe_term_eta_expand_aux. Qed.
-
-Lemma decompose_app_rec_app t acc acc' :
-  let (hd, args) := decompose_app_rec t acc in
-  decompose_app_rec t (acc ++ acc') = (hd, args ++ acc').
-Proof.
-  revert acc.
-  induction t using term_forall_list_ind; intros acc; try easy.
-  cbn.
-  specialize (IHt1 (t2 :: acc)).
-  now rewrite <- app_comm_cons in IHt1.
-Qed.
-
-Lemma eta_expand_aux_unfold t args :
-  eta_expand_aux args t =
-  match decompose_app t with
-  | (tConstruct ind c, args') => eta_ctor ind c (map (eta_expand_aux []) args' ++ args)
-  | (tConst kn, args') => eta_const kn (map (eta_expand_aux []) args' ++ args)
-  | (hd, args') => mkApps
-                     (map_subterms (eta_expand_aux []) hd)
-                     (map (eta_expand_aux []) args' ++ args)
-  end.
-Proof.
-  revert args.
-  induction t using term_forall_list_ind; intros args; cbn in *;
-    try easy.
-  rewrite IHt1.
-  unfold decompose_app.
-  pose proof (decompose_app_rec_app t1 [] [t2]).
-  destruct (decompose_app_rec t1 []) as [hd args'].
-  cbn in *.
-  rewrite H.
-  rewrite map_app.
-  cbn.
-  now rewrite <- app_assoc.
-Qed.
-
-Lemma eta_expand_unfold t :
-  eta_expand t =
-  match decompose_app t with
-  | (tConstruct ind c, args) => eta_ctor ind c (map eta_expand args)
-  | (tConst kn, args) => eta_const kn (map eta_expand args)
-  | (hd, args) => mkApps (map_subterms eta_expand hd) (map eta_expand args)
-  end.
-Proof.
-  unfold eta_expand at 1.
-  rewrite eta_expand_aux_unfold.
-  destruct (decompose_app _).
-  now rewrite app_nil_r.
-Qed.
-
-End eta_correctness.
-*)
 
 Section dearg_correctness.
 Context (ind_masks : list (kername * mib_masks)).
@@ -505,430 +333,6 @@ Proof.
   now rewrite List.rev_involutive.
 Qed.
 
-(*
-Lemma subst_context_app Γ Γ' inner args :
-  #|vasses Γ'| <= #|args| ->
-  subst_context (Γ ++ Γ') inner args =
-  subst_context Γ (subst_context Γ' inner args) (skipn #|vasses Γ'| args).
-Proof.
-  intros len.
-  unfold subst_context.
-  rewrite List.rev_app_distr.
-  rewrite subst_context_aux_app.
-  - now rewrite vasses_rev, List.rev_length.
-  - now rewrite vasses_rev, List.rev_length.
-Qed.
-
-Lemma subst_context_aux_enough_args Γ inner args :
-  subst_context_aux Γ inner args =
-  subst_context_aux Γ inner (firstn #|vasses Γ| args).
-Proof.
-  revert inner args.
-  induction Γ; intros inner args; [easy|].
-  cbn.
-  refold.
-  destruct (decl_body a).
-  - easy.
-  - destruct args; [easy|].
-    apply IHΓ.
-Qed.
-
-Lemma subst_context_enough_args Γ inner args :
-  subst_context Γ inner args =
-  subst_context Γ inner (firstn #|vasses Γ| args).
-Proof.
-  unfold subst_context.
-  replace #|vasses Γ| with #|vasses (List.rev Γ)|.
-  - apply subst_context_aux_enough_args.
-  - now rewrite vasses_rev, List.rev_length.
-Qed.
-
-Lemma firstn_all_app_eq {A} n (l l' : list A) :
-  n = #|l| ->
-  firstn n (l ++ l') = l.
-Proof.
-  intros ->.
-  replace #|l| with (#|l| + 0) by lia.
-  rewrite firstn_app_2.
-  cbn.
-  apply app_nil_r.
-Qed.
-*)
-
-Derive Signature for eval.
-Derive NoConfusionHom for term.
-
-Lemma eval_tLetIn Σ na val body res :
-  Σ ⊢ tLetIn na val body ▷ res ->
-  exists val_res,
-    Σ ⊢ val ▷ val_res /\
-    Σ ⊢ csubst val_res 0 body ▷ res.
-Proof.
-  intros ev.
-  depind ev; try easy.
-  - destruct args using List.rev_ind; [easy|].
-    rewrite mkApps_app in *.
-    cbn in *.
-    congruence.
-  - destruct args using List.rev_ind.
-    + cbn in *.
-      depelim H.
-      subst f.
-      now eapply IHev.
-    + rewrite mkApps_app in *.
-      cbn in *.
-      congruence.
-Qed.
-
-Inductive head_of_app_cases : term -> Prop :=
-| head_box : head_of_app_cases tBox
-| head_lambda na body : head_of_app_cases (tLambda na body)
-| head_fix defs f args :
-    isStuckFix (tFix defs f) args ->
-    Forall value args ->
-    head_of_app_cases (mkApps (tFix defs f) args)
-| head_cofix defs f args :
-    Forall value args ->
-    head_of_app_cases (mkApps (tCoFix defs f) args)
-| head_ctor ind c args :
-    Forall value args ->
-    head_of_app_cases (mkApps (tConstruct ind c) args).
-
-Lemma eval_tApp_inv Σ hd arg v :
-  Σ ⊢ tApp hd arg ▷ v ->
-  exists hdv argv,
-    Σ ⊢ hd ▷ hdv /\
-    Σ ⊢ arg ▷ argv /\
-    head_of_app_cases hdv.
-Proof.
-  intros ev.
-  depind ev.
-  - exists tBox, t'.
-    split; [easy|].
-    split; [easy|].
-    now constructor.
-  - exists (tLambda na b), a'.
-    split; [easy|].
-    split; [easy|].
-    now constructor.
-  - destruct args using List.rev_ind; [easy|].
-    clear IHargs.
-    rewrite mkApps_app in H3.
-    cbn in *.
-    apply Forall2_length in H2 as args_len.
-    rewrite !app_length in *.
-    cbn in *.
-    destruct args' as [|a' args' _] using List.rev_ind; [cbn in *; abstract lia|].
-    exists (mkApps (tFix mfix idx) args'), a'.
-    inversion H3; subst; clear H3.
-    assert (stuck: isStuckFix (tFix mfix idx) args').
-    {unfold isStuckFix, cunfold_fix, ETyping.unfold_fix in *.
-     destruct (nth_error mfix idx) as [f'|]; [|easy].
-     replace (rarg f') with narg by congruence.
-     unfold ETyping.is_constructor.
-     rewrite !app_length in *.
-     cbn in *.
-     rewrite (proj2 (nth_error_None _ _)) by abstract lia.
-     easy. }
-    split; [|split].
-    + apply eval_fix_value.
-      * easy.
-      * apply Forall2_app_r in H2.
-        easy.
-      * easy.
-    + now apply Forall2_app_r in H2.
-    + constructor; [easy|].
-      apply Forall2_app_r in H2.
-      destruct H2 as (all_eval & _).
-      clear -all_eval.
-      induction all_eval; [easy|].
-      constructor; [|easy].
-      now eapply eval_to_value.
-  - destruct args as [|a args _] using List.rev_ind.
-    + cbn in *.
-      eapply IHev.
-      now f_equal.
-    + rewrite mkApps_app in H1.
-      apply Forall2_length in H as args_len.
-      rewrite !app_length in *.
-      cbn in *.
-      destruct args' as [|a' args' _] using List.rev_ind; [cbn in *; abstract lia|].
-      exists (mkApps (tFix mfix idx) args'), a'.
-      inversion H1; subst; clear H1.
-      assert (stuck: isStuckFix (tFix mfix idx) args').
-      { unfold isStuckFix.
-        destruct (ETyping.unfold_fix mfix idx) as [(? & ?)|]; [|easy].
-        unfold ETyping.is_constructor in H0.
-        destruct (Nat.ltb_spec n #|args'|).
-        - rewrite nth_error_app_lt in H0 by easy.
-          apply H0.
-        - unfold ETyping.is_constructor.
-          now rewrite (proj2 (nth_error_None _ _)) by abstract lia. }
-      split; [|split].
-      * apply eval_fix_value; [easy| |easy].
-        now apply Forall2_app_r in H.
-      * now apply Forall2_app_r in H.
-      * constructor; [easy|].
-        apply Forall2_app_r in H.
-        destruct H as (all_eval & _).
-        clear -all_eval.
-        induction all_eval; [easy|].
-        constructor; [|easy].
-        now eapply eval_to_value.
-  - exists f', a'.
-    split; [easy|].
-    split; [easy|].
-    apply eval_to_value in ev1 as f'value.
-    destruct f'value.
-    + destruct t; cbn in *; try congruence.
-      * now apply (head_ctor _ _ []).
-      * now apply (head_cofix _ _ []).
-    + destruct t; cbn in *; try congruence.
-      * now constructor.
-      * now constructor.
-    + clear -H1 H.
-      exfalso.
-      destruct f0; try easy.
-      propize.
-      destruct H as ((_ & not_fix) & _).
-      now rewrite isFixApp_mkApps in not_fix.
-  - easy.
-Qed.
-
-Lemma eval_tApp_head Σ hd arg v :
-  Σ ⊢ tApp hd arg ▷ v ->
-  exists hdv, Σ ⊢ hd ▷ hdv /\ head_of_app_cases hdv.
-Proof.
-  intros ev.
-  now destruct (eval_tApp_inv Σ hd arg v ev) as (? & ? & ?).
-Qed.
-
-Lemma eval_tApp_arg Σ hd arg v :
-  Σ ⊢ tApp hd arg ▷ v ->
-  exists argv, Σ ⊢ arg ▷ argv.
-Proof.
-  intros ev.
-  now destruct (eval_tApp_inv Σ hd arg v ev) as (? & ? & ?).
-Qed.
-
-Lemma eval_mkApps_inv Σ hd args v :
-  Σ ⊢ mkApps hd args ▷ v ->
-  exists hdv argsv,
-    Σ ⊢ hd ▷ hdv /\
-    Forall2 (eval Σ) args argsv /\
-    (args = [] \/ head_of_app_cases hdv).
-Proof.
-  revert hd v.
-  induction args; intros hd v ev.
-  - cbn in *.
-    now exists v, [].
-  - cbn in *.
-    specialize (IHargs _ _ ev).
-    destruct IHargs as (app_hdv & app_argsv & ev_app & ? & ?).
-    apply eval_tApp_inv in ev_app.
-    destruct ev_app as (hdv & argv & ev_hd & ev_arg & head_hdv).
-    exists hdv, (argv :: app_argsv).
-    easy.
-Qed.
-
-Lemma eval_mkApps_head Σ hd args v :
-  Σ ⊢ mkApps hd args ▷ v ->
-  exists hdv, Σ ⊢ hd ▷ hdv /\ (args = [] \/ head_of_app_cases hdv).
-Proof.
-  intros ev.
-  destruct (eval_mkApps_inv _ _ _ _ ev) as (? & ? & ? & ? & ?).
-  eexists.
-  easy.
-Qed.
-
-Lemma eval_mkApps_args Σ hd args v :
-  Σ ⊢ mkApps hd args ▷ v ->
-  exists argsv, Forall2 (eval Σ) args argsv.
-Proof.
-  intros ev.
-  now destruct (eval_mkApps_inv _ _ _ _ ev) as (? & ? & ?).
-Qed.
-
-Ltac gen_equalities :=
-  repeat
-    match goal with
-    | [H: ?Σ ⊢ ?a ▷ ?v, IH: forall _ : term, ?Σ ⊢ ?a ▷ _ -> _ |- _ = _] =>
-      let t := constr:(IH _ H) in
-      let tty := type of t in
-      (match goal with
-       | [H: tty |- _] => fail 2
-       end || pose proof t)
-    end;
-  repeat
-    match goal with
-    | [H: ?a = ?a |- _] => clear H
-    end.
-
-Lemma eval_deterministic Σ t v v' :
-  Σ ⊢ t ▷ v ->
-  Σ ⊢ t ▷ v' ->
-  v = v'.
-Proof.
-  intros ev1.
-  revert v'.
-  induction ev1 using eval_evals_ind; intros v' ev2.
-  - admit.
-  - apply eval_tApp_inv in ev2.
-    destruct ev2 as (hdv & argv & ev_hd & ev_arg & hd_app).
-    inversion hd_app; subst; clear hd_app;
-      gen_equalities; try congruence; try solve_discr.
-    inversion H2; subst.
-    admit.
-  - apply eval_tLetIn in ev2.
-    destruct ev2 as (? & ? & ?).
-    gen_equalities.
-    subst.
-    now gen_equalities.
-  - depind ev2.
-    + destruct args using List.rev_ind; [easy|].
-      now rewrite mkApps_app in H5.
-    + destruct args using List.rev_ind; [|now rewrite mkApps_app in *].
-      cbn in *.
-      subst f.
-      apply Forall2_length in H.
-      destruct args'; [|easy].
-      cbn in *.
-      eapply IHev2; easy.
-    + unfold ETyping.declared_constant in *.
-      replace body0 with body in * by congruence.
-      now gen_equalities.
-    + easy.
-  - depind ev2.
-    + gen_equalities.
-      solve_discr.
-      inversion H; subst; clear H.
-      now gen_equalities.
-    + gen_equalities.
-      solve_discr.
-    + destruct args using List.rev_ind; [easy|].
-      rewrite mkApps_app in H3.
-      solve_discr.
-    + destruct args using List.rev_ind; cycle 1.
-      { now rewrite mkApps_app in H1. }
-      cbn in *.
-      subst f.
-      apply Forall2_length in H.
-      destruct args'; [|easy].
-      cbn in *.
-      easy.
-    + admit.
-    + easy.
-  - depind ev2; subst.
-    + gen_equalities.
-      solve_discr.
-    + inversion H; subst.
-      now gen_equalities.
-    + destruct args using List.rev_ind; [easy|].
-      now rewrite mkApps_app in *.
-    + destruct args using List.rev_ind; cycle 1.
-      { now rewrite mkApps_app in H1. }
-      cbn in *.
-      subst f.
-      apply Forall2_length in H.
-      destruct args'; [|easy].
-      easy.
-    + apply eval_mkApps_inv in ev1_1.
-      destruct ev1_1 as (hdv & argsv & ev_hd & ev_args & disc).
-      destruct disc as [->|].
-      * cbn in *.
-        gen_equalities.
-        subst.
-        assert (Σ ⊢ tCoFix mfix idx ▷ tCoFix mfix idx); [|gen_equalities; easy].
-        now apply eval_atom.
-      * admit.
-    + easy.
-  - admit.
-  - admit.
-  - admit.
-  - admit.
-  - admit.
-    assert (Σ ⊢ tProj (i, pars, arg) discr ▷ tBox).
-    { now apply eval_proj_box. }
-    gen_equalities.
-      eapply IHev2
-      subst brs.
-      cbn in *.
-      easy.
-      apply IHev1.
-      subst f.
-      2: {
-      gen_equalities; try congruence; try solve_discr.
-
-    +
-    + gen_equalities; congruence.
-    + gen_equalities; subst.
-      inversion H2; subst.
-      gen_equalities.
-      admit.
-    + gen_equalities.
-      solve_discr.
-    + gen_equalities.
-      solve_discr.
-    + gen_equai
-    depelim ev2.
-    + gen_equalities; congruence.
-    + gen_equalities.
-      inversion H2.
-      subst.
-      now gen_equalities.
-    + destruct args as [|a'' args _] using List.rev_ind; [easy|].
-      rewrite mkApps_app in H3.
-      cbn in *.
-      inversion H3; subst; clear H3.
-
-      replace f with (mkApps f0 args) in * by congruence.
-      apply eval_mkApps_inv in ev2_2.
-      destruct ev2_2 as (? & ? & ? & ? & ?).
-
-      gen_equalities.
-      subst a'0.
-      inversion H2; subst; clear H2.
-      apply IHev1_3.
-      let x := (has_hypothesis_of_type term) in
-      match x with
-      | 0 => idtac "foo"
-      | 1 => idtac "bar"
-      end.
-      gen_equalities.
-      gen_equalities.
-    +
-    apply eval_tApp_inv in ev2 as (hdv & argv & ev_hd & ev_arg & hd_cases).
-    apply IHev1_3.
-    depelim hd_cases; try solve_congr.
-    + apply IHev1_3.
-    +
-    inversion hd_cases; subst.
-    apply eval_tApp_head in ev2.
-    destruct ev2 as (hdv & ev_hd & hdv_cases).
-    depelim hdv_cases;
-      specialize (IHev1_1 _ ev_hd); try congruence.
-
-(*
-Lemma eval_tLambda_to_tBox Σ na body :
-  Σ ⊢ tLambda na body ▷ tBox ->
-  False.
-Proof.
-  intros.
-  depelim H.
-  - destruct args using List.rev_ind; [easy|now rewrite mkApps_app in *].
-  - destruct args' using List.rev_ind; [easy|now rewrite mkApps_app in *].
-Qed.
-
-Lemma eval_tApp_tLambda Σ na body hd v :
-  Σ ⊢ tApp (tLambda na body) hd ▷ v ->
-  Σ ⊢ csubst hd 0 body ▷ v.
-Proof.
-  intros.
-  depelim H.
-  - now apply eval_tLambda_to_tBox in H.
-  - easy.
-*)
-
 Fixpoint subst_in_let_values (ts : list term) (k : nat) (Γ : context) : context :=
   match Γ with
   | [] => []
@@ -1110,29 +514,29 @@ Proof.
   revert k n.
   induction t using term_forall_list_ind; intros k n' clos klen;
     cbn in *; auto.
-  - propize.
+  - propify.
     destruct (Nat.eqb_spec n n'); lia.
   - induction H; [easy|].
     cbn in *.
-    propize.
+    propify.
     easy.
   - easy.
-  - propize.
+  - propify.
     easy.
-  - propize.
+  - propify.
     easy.
-  - propize.
+  - propify.
     induction X; [easy|].
     destruct x.
     cbn in *.
-    propize.
+    propify.
     easy.
   - easy.
   - revert k n' clos klen.
     induction H; [easy|]; intros k n' clos klen.
     destruct x.
     cbn in *.
-    propize.
+    propify.
     split; [easy|].
     replace (n' + S #|l|) with (S n' + #|l|) by abstract lia.
     apply (IHForall (S k)); [|easy].
@@ -1141,7 +545,7 @@ Proof.
     induction H; [easy|]; intros k n' clos klen.
     destruct x.
     cbn in *.
-    propize.
+    propify.
     split; [easy|].
     replace (n' + S #|l|) with (S n' + #|l|) by abstract lia.
     apply (IHForall (S k)); [|easy].
@@ -1157,40 +561,40 @@ Proof.
   revert k u k'.
   induction t using term_forall_list_ind; intros k u k' use_eq clos kltn;
     cbn in *; auto.
-  - propize.
+  - propify.
     destruct (Nat.compare_spec k' n) as [->| |].
     + now apply has_use_closed with k.
     + cbn.
-      propize.
+      propify.
       lia.
     + cbn.
-      propize.
+      propify.
       lia.
   - induction H; [easy|].
     cbn in *.
-    propize.
+    propify.
     easy.
-  - propize.
+  - propify.
     apply IHt; [easy| |easy].
     now eapply closed_upwards.
-  - propize.
+  - propify.
     split; [easy|].
     apply IHt2; [easy| |easy].
     now eapply closed_upwards.
-  - propize.
+  - propify.
     split; [easy|].
     apply IHt2; [easy| |easy].
     now eapply closed_upwards.
   - induction X; [easy|].
     destruct x.
     cbn in *.
-    propize.
+    propify.
     easy.
   - revert k k' kltn use_eq clos.
     induction H; [easy|]; intros k k' kltn use_eq clos.
     destruct x.
     cbn in *.
-    propize.
+    propify.
     rewrite map_length in *.
     split.
     + apply H; [easy| |easy].
@@ -1204,7 +608,7 @@ Proof.
     induction H; [easy|]; intros k k' kltn use_eq clos.
     destruct x.
     cbn in *.
-    propize.
+    propify.
     rewrite map_length in *.
     split.
     + apply H; [easy| |easy].
@@ -1217,40 +621,6 @@ Proof.
 Qed.
 
 (*
-Lemma closedn_subst s k k' t :
-  forallb (closedn k) s -> closedn (k + k' + #|s|) t ->
-  closedn (k + k') (subst s k' t).
-Proof.
-  intros Hs. solve_all. revert H.
-  induction t in k' |- * using term_forall_list_ind; intros;
-    simpl in *;
-    rewrite -> ?map_map_compose, ?compose_on_snd, ?compose_map_def, ?map_length;
-    simpl closed in *; try change_Sk; repeat (rtoProp; solve_all);
-    unfold compose, test_def, on_snd, test_snd in *; simpl in *; eauto with all.
-
-  - elim (Nat.leb_spec k' n); intros. simpl.
-    apply Nat.ltb_lt in H.
-    destruct nth_error eqn:Heq.
-    -- eapply closedn_lift.
-       now eapply nth_error_all in Heq; simpl; eauto; simpl in *.
-    -- simpl. elim (Nat.ltb_spec); auto. intros.
-       apply nth_error_None in Heq. lia.
-    -- simpl. apply Nat.ltb_lt in H0.
-       apply Nat.ltb_lt. apply Nat.ltb_lt in H0. lia.
-
-  - specialize (IHt2 (S k')).
-    rewrite <- Nat.add_succ_comm in IHt2. eauto.
-  - specialize (IHt2 (S k')).
-    rewrite <- Nat.add_succ_comm in IHt2. eauto.
-  - specialize (IHt3 (S k')).
-    rewrite <- Nat.add_succ_comm in IHt3. eauto.
-  - rtoProp; solve_all. rewrite -> !Nat.add_assoc in *.
-    specialize (b0 (#|m| + k')). unfold is_true. rewrite <- b0. f_equal. lia.
-    unfold is_true. rewrite <- H0. f_equal. lia.
-  - rtoProp; solve_all. rewrite -> !Nat.add_assoc in *.
-    specialize (b0 (#|m| + k')). unfold is_true. rewrite <- b0. f_equal. lia.
-    unfold is_true. rewrite <- H0. f_equal. lia.
-Qed.
 
 Lemma closedn_subst0 s k t :
   forallb (closedn k) s -> closedn (k + #|s|) t ->
@@ -1263,9 +633,6 @@ Qed.
 *)
 
 
-Lemma closed_csubst t k u : closed t -> closedn (S k) u -> closedn k (csubst t 0 u).
-Proof.
-  Admitted.
 (*
   intros.
   rewrite closed_subst; auto.
@@ -1274,170 +641,6 @@ Proof.
 Qed.
 *)
 
-Lemma closed_mkApps hd args :
-  closed hd ->
-  Forall (closedn 0) args ->
-  closed (mkApps hd args).
-Proof.
-  revert hd.
-  induction args using List.rev_ind; [easy|].
-  intros hd closed_hd closed_args.
-  rewrite mkApps_app.
-  cbn.
-  propize.
-  apply Forall_app in closed_args.
-  destruct closed_args as (? & closed_x).
-  split; [|now inversion closed_x].
-  easy.
-Qed.
-
-Lemma closed_mkApps_inv hd args :
-  closed (mkApps hd args) ->
-  closed hd /\
-  Forall (closedn 0) args.
-Proof.
-  revert hd.
-  induction args using List.rev_ind; [easy|]; intros hd clos.
-  rewrite mkApps_app in clos.
-  cbn in clos.
-  propize.
-  specialize (IHargs hd ltac:(easy)).
-  split; [easy|].
-  apply app_Forall; [easy|].
-  constructor; easy.
-Qed.
-
-Lemma closed_mkApps_head hd args :
-  closed (mkApps hd args) ->
-  closed hd.
-Proof.
-  intros clos.
-  now pose proof (closed_mkApps_inv _ _ clos).
-Qed.
-
-Lemma closed_mkApps_args hd args :
-  closed (mkApps hd args) ->
-  Forall (closedn 0) args.
-Proof.
-  intros clos.
-  now pose proof (closed_mkApps_inv _ _ clos).
-Qed.
-
-Definition decl_closed (decl : EAst.global_decl) : Prop :=
-  match decl with
-  | EAst.ConstantDecl cst =>
-    match EAst.cst_body cst with
-    | Some body => closed body
-    | _ => True
-    end
-  | _ => True
-  end.
-
-Lemma mclookup_env_find Σ kn :
-  ETyping.lookup_env Σ kn =
-  option_map snd (find (fun '(kn', _) => if kername_eq_dec kn kn' then true else false) Σ).
-Proof.
-  induction Σ as [|(kn' & decl) Σ IH]; [easy|].
-  cbn.
-  now destruct (kername_eq_dec kn kn').
-Qed.
-
-Definition env_closed (Σ : EAst.global_declarations) :=
-  Forall (decl_closed ∘ snd) Σ.
-
-Lemma closed_constant Σ kn cst :
-  env_closed Σ ->
-  ETyping.declared_constant Σ kn cst ->
-  match EAst.cst_body cst with
-  | Some val => closed val = true
-  | None => True
-  end.
-Proof.
-  intros env_clos decl_const.
-  unfold ETyping.declared_constant in decl_const.
-  rewrite mclookup_env_find in decl_const.
-  destruct (find _ _) eqn:find; [|easy].
-  apply find_some in find.
-  unfold env_closed in env_clos.
-  rewrite Forall_forall in env_clos.
-  specialize (env_clos _ (proj1 find)).
-  destruct p.
-  cbn in *.
-  now inversion decl_const; subst.
-Qed.
-
-Lemma eval_closed Σ t v :
-  env_closed Σ ->
-  closed t ->
-  Σ ⊢ t ▷ v ->
-  closed v.
-Proof.
-  intros env_clos clos ev.
-  induction ev using eval_evals_ind; cbn in *.
-  - easy.
-  - propize.
-    apply IHev3.
-    now apply closed_csubst.
-  - propize.
-    apply IHev2.
-    now apply closed_csubst.
-  - apply IHev.
-    pose proof (closed_constant _ _ _ env_clos H).
-    now rewrite H0 in *.
-  - propize.
-    apply IHev2.
-    unfold ETyping.iota_red.
-    apply closed_mkApps.
-    + destruct clos as (_ & clos).
-      clear -clos.
-      revert c.
-      induction brs; intros c.
-      * now rewrite nth_nth_error, nth_error_nil.
-      * cbn in *.
-        propize.
-        now destruct a, c.
-    + apply Forall_skipn.
-      eapply closed_mkApps_args.
-      apply IHev1.
-      easy.
-  - subst brs.
-    cbn in *.
-    propize.
-    apply IHev2.
-    apply closed_mkApps; [easy|].
-    clear.
-    induction n; [constructor|].
-    constructor; easy.
-  - apply IHev2.
-    specialize (IHev1 clos).
-    apply closed_mkApps_args in IHev1.
-    rewrite nth_nth_error in *.
-    destruct (nth_error _ _) eqn:nth_eq.
-    + apply nth_error_In in nth_eq.
-      now rewrite Forall_forall in IHev1.
-    + easy.
-  - easy.
-  - apply IHev2.
-    specialize (IHev1 (closed_mkApps_head _ _ clos)).
-    apply closed_mkApps.
-    + apply forallb_Forall in IHev1.
-      unfold cunfold_fix in H.
-      destruct (nth_error mfix idx) eqn:nth_eq; [|easy].
-      apply nth_error_In in nth_eq.
-      rewrite Forall_forall in IHev1.
-      exact (todo "Fixpoint unfold").
-    + exact (todo "Fixpoint args").
-  - apply closed_mkApps.
-    + cbn.
-      apply IHev.
-      now eapply closed_mkApps_head.
-    + exact (todo "Stuck fixpoint unfold").
-  - exact (todo "CoFix").
-  - exact (todo "CoFix").
-  - propize.
-    easy.
-  - easy.
-Qed.
 
 Lemma valid_dearg_mask_nil t : valid_dearg_mask [] t.
 Proof. induction t; easy. Qed.
@@ -1460,6 +663,29 @@ Proof.
     + now apply IHt.
 Qed.
 
+Lemma valid_dearg_mask_app mask mask' Γ inner :
+  valid_dearg_mask (mask ++ mask') (it_mkLambda_or_LetIn Γ inner) ->
+  #|vasses Γ| = #|mask| ->
+  valid_dearg_mask mask' inner.
+Proof.
+  revert mask mask' inner.
+  induction Γ as [|cd Γ IH] using List.rev_ind; intros mask mask' inner len_eq valid_mask.
+  - destruct mask; [|easy].
+    easy.
+  - rewrite it_mkLambda_or_LetIn_app, vasses_app, app_length in *.
+    cbn in *.
+    unfold mkLambda_or_LetIn in *.
+    destruct (decl_body cd) eqn:decl_eq.
+    + cbn in *.
+      easy.
+    + cbn in *.
+      destruct mask; [now cbn in *|].
+      cbn in *.
+      destruct b.
+      * now eapply IH.
+      * easy.
+Qed.
+
 Lemma valid_dearg_mask_eval_lambdas mask body Σ args t :
   valid_dearg_mask mask body ->
   #|args| = #|mask| ->
@@ -1476,10 +702,34 @@ Proof.
     easy.
   - rewrite mkApps_app in ev.
     cbn in *.
-    destruct mask as [|b mask _] using List.rev_ind.
+    destruct mask as [|b mask].
     { now rewrite app_length in len_eq; cbn in *. }
+    cbn in *.
+    apply Forall_app in all_closed.
+    rewrite List.rev_app_distr, app_length in *.
+    destruct body; try easy.
+    + cbn in *.
+      exists n, body.
+      split; [apply eval_atom; easy|].
+      apply eval_tApp_inv in ev as (hdv & argv & ? & ? & ?).
+      eapply eval_lambdas_tApp_tLambda; [easy|].
+      apply (IHargs mask _ hdv).
+      * apply valid_dearg_mask_csubst; [easy|].
+        eapply eval_closed; [eassumption| |easy].
+        now destruct all_closed as (_ & clos); inversion clos.
+      * lia.
+      * easy.
+      *
     rewrite List.rev_app_distr.
     cbn.
+    destruct (valid_dearg_mask_spec (mask ++ [b]) body)
+      as (Γ & inner & len_eq' & body_eq); [easy|].
+    rewrite body_eq in valid_mask.
+    rewrite app_length in len_eq'.
+    induction Γ using List.rev_ind; [now cbn in *|].
+    rewrite it_mkLambda_or_LetIn_app in *.
+    cbn in valid_mask.
+    + cbn in *.
     destruct body; try easy.
     + cbn in *.
       exists n, body.
