extraction/theories/Aux.v
@@ -1,0 +1,31 @@
+From Coq Require Import Arith.
+From Coq Require Import Bool.
+From Coq Require Import List.
+From Equations Require Import Equations.
+
+Derive Signature for Forall.
+Derive Signature for Forall2.
+
+Ltac propify :=
+  unfold is_true in *;
+  repeat
+    match goal with
+    | [H: context[orb _ _ = false] |- _] => rewrite Bool.orb_false_iff in H
+    | [H: context[orb _ _ = true] |- _] => rewrite Bool.orb_true_iff in H
+    | [|- context[orb _ _ = false]] => rewrite Bool.orb_false_iff
+    | [|- context[orb _ _ = true]] => rewrite Bool.orb_true_iff
+    | [H: context[andb _ _ = false] |- _] => rewrite Bool.andb_false_iff in H
+    | [H: context[andb _ _ = true] |- _] => rewrite Bool.andb_true_iff in H
+    | [H: context[negb _ = true] |- _] => rewrite Bool.negb_true_iff in H
+    | [H: context[negb _ = false] |- _] => rewrite Bool.negb_false_iff in H
+    | [|- context[andb _ _ = false]] => rewrite Bool.andb_false_iff
+    | [|- context[andb _ _ = true]] => rewrite Bool.andb_true_iff
+    | [H: context[Nat.ltb _ _ = true] |- _] => rewrite Nat.ltb_lt in H
+    | [H: context[Nat.ltb _ _ = false] |- _] => rewrite Nat.ltb_ge in H
+    | [|- context[Nat.ltb _ _ = true]] => rewrite Nat.ltb_lt
+    | [|- context[Nat.ltb _ _ = false]] => rewrite Nat.ltb_ge
+    | [H: context[Nat.eqb _ _ = true] |- _] => rewrite Nat.eqb_eq in H
+    | [H: context[Nat.eqb _ _ = false] |- _] => rewrite Nat.eqb_neq in H
+    | [|- context[Nat.eqb _ _ = true]] => rewrite Nat.eqb_eq
+    | [|- context[Nat.eqb _ _ = false]] => rewrite Nat.eqb_neq
+    end.
