extraction/theories/ClosedAux.v
@@ -1,0 +1,189 @@
+From ConCert.Extraction Require Import Aux.
+From Coq Require Import Arith.
+From Coq Require Import Bool.
+From Coq Require Import List.
+From Coq Require Import Psatz.
+From Equations Require Import Equations.
+From MetaCoq.Erasure Require Import EAst.
+From MetaCoq.Erasure Require Import EAstUtils.
+From MetaCoq.Erasure Require Import ECSubst.
+From MetaCoq.Erasure Require Import EInduction.
+From MetaCoq.Erasure Require Import ELiftSubst.
+From MetaCoq.Erasure Require Import EWcbvEval.
+From MetaCoq.Template Require Import utils.
+
+Import ListNotations.
+Set Equations Transparent.
+
+Lemma closed_mkApps hd args :
+  closed hd ->
+  Forall (closedn 0) args ->
+  closed (mkApps hd args).
+Proof.
+  revert hd.
+  induction args using List.rev_ind; [easy|].
+  intros hd closed_hd closed_args.
+  rewrite mkApps_app.
+  cbn.
+  propify.
+  apply Forall_app in closed_args.
+  destruct closed_args as (? & closed_x).
+  split; [|now inversion closed_x].
+  easy.
+Qed.
+
+Lemma closed_mkApps_inv hd args :
+  closed (mkApps hd args) ->
+  closed hd /\
+  Forall (closedn 0) args.
+Proof.
+  revert hd.
+  induction args using List.rev_ind; [easy|]; intros hd clos.
+  rewrite mkApps_app in clos.
+  cbn in clos.
+  propify.
+  specialize (IHargs hd ltac:(easy)).
+  split; [easy|].
+  apply app_Forall; [easy|].
+  constructor; easy.
+Qed.
+
+Lemma closed_mkApps_head hd args :
+  closed (mkApps hd args) ->
+  closed hd.
+Proof.
+  intros clos.
+  now pose proof (closed_mkApps_inv _ _ clos).
+Qed.
+
+Lemma closed_mkApps_args hd args :
+  closed (mkApps hd args) ->
+  Forall (closedn 0) args.
+Proof.
+  intros clos.
+  now pose proof (closed_mkApps_inv _ _ clos).
+Qed.
+
+Definition decl_closed (decl : EAst.global_decl) : Prop :=
+  match decl with
+  | EAst.ConstantDecl cst =>
+    match EAst.cst_body cst with
+    | Some body => closed body
+    | _ => True
+    end
+  | _ => True
+  end.
+
+Arguments Nat.ltb : simpl nomatch.
+
+Lemma closedn_lift n k k' t : closedn k t -> closedn (k + n) (lift n k' t).
+Proof.
+  revert n k k'.
+  induction t using term_forall_list_ind; intros n' k k' clos;
+    cbn in *; auto; propify.
+  - destruct (Nat.leb_spec k' n);
+      cbn; propify; lia.
+  - induction H; cbn in *; propify; easy.
+  - erewrite <- IHt by eassumption.
+    easy.
+  - erewrite <- IHt1 at 1 by easy.
+    erewrite <- IHt2 by easy.
+    easy.
+  - easy.
+  - split; [easy|].
+    destruct clos as (_ & clos).
+    induction X; cbn in *; propify; easy.
+  - rewrite map_length.
+    revert n' k k' clos.
+    induction H; intros n' k k' clos; cbn in *; propify; [easy|].
+    destruct x; cbn in *.
+    split.
+    + erewrite <- (H _ (S (#|l| + k)) _) by easy.
+      f_equal.
+      lia.
+    + erewrite <- (IHForall n' (S k) (S k'));
+        repeat (f_equal; try lia).
+      rewrite <- (proj2 clos);
+        repeat (f_equal; try lia).
+  - rewrite map_length.
+    revert n' k k' clos.
+    induction H; intros n' k k' clos; cbn in *; propify; [easy|].
+    destruct x; cbn in *.
+    split.
+    + erewrite <- (H _ (S (#|l| + k)) _) by easy.
+      f_equal.
+      lia.
+    + erewrite <- (IHForall n' (S k) (S k'));
+        repeat (f_equal; try lia).
+      rewrite <- (proj2 clos);
+        repeat (f_equal; try lia).
+Qed.
+
+Lemma closedn_subst s k k' t :
+  Forall (closedn k) s -> closedn (k + k' + #|s|) t ->
+  closedn (k + k') (subst s k' t).
+Proof.
+  revert k k'.
+  induction t using term_forall_list_ind; intros k k' all clos;
+    cbn in *; auto; propify.
+  - destruct (Nat.leb_spec k' n); cbn in *; propify.
+    + destruct nth_error eqn:eq;
+        cbn in *.
+      * apply closedn_lift.
+        rewrite Forall_forall in all.
+        apply nth_error_In in eq.
+        easy.
+      * propify.
+        apply nth_error_None in eq.
+        lia.
+    + lia.
+  - induction H; cbn in *; propify; easy.
+  - erewrite <- (IHt _ (S k')); [|easy|rewrite <- clos; f_equal; lia].
+    f_equal; lia.
+  - split; [easy|].
+    erewrite <- (IHt2 _ (S k')); [|easy|].
+    + f_equal; lia.
+    + rewrite <- (proj2 clos); f_equal; lia.
+  - easy.
+  - split; [easy|].
+    induction X; cbn in *; propify; easy.
+  - rewrite map_length.
+    revert k k' all clos.
+    induction H; intros k k' all all'; cbn in *; propify; [easy|].
+    destruct x; cbn in *.
+    split.
+    + erewrite <- (H _ (S (#|l| + k'))); [|easy|].
+      * f_equal; lia.
+      * rewrite <- (proj1 all').
+        f_equal; lia.
+    + erewrite <- (IHForall _ (S k')); [|easy|].
+      * repeat (f_equal; try lia).
+      * rewrite <- (proj2 all').
+        repeat (f_equal; try lia).
+  - rewrite map_length.
+    revert k k' all clos.
+    induction H; intros k k' all all'; cbn in *; propify; [easy|].
+    destruct x; cbn in *.
+    split.
+    + erewrite <- (H _ (S (#|l| + k'))); [|easy|].
+      * f_equal; lia.
+      * rewrite <- (proj1 all').
+        f_equal; lia.
+    + erewrite <- (IHForall _ (S k')); [|easy|].
+      * repeat (f_equal; try lia).
+      * rewrite <- (proj2 all').
+        repeat (f_equal; try lia).
+Qed.
+
+Lemma lookup_env_find Σ kn :
+  ETyping.lookup_env Σ kn =
+  option_map snd (find (fun '(kn', _) => if kername_eq_dec kn kn' then true else false) Σ).
+Proof.
+  induction Σ as [|(kn' & decl) Σ IH]; [easy|].
+  cbn.
+  now destruct (kername_eq_dec kn kn').
+Qed.
+
+Lemma closed_csubst t k u : closed t -> closedn (S k) u -> closedn k (csubst t 0 u).
+Proof.
+  Admitted.
