extraction/theories/WcbvEvalAux.v
@@ -1,0 +1,508 @@
+From ConCert.Extraction Require Import Aux.
+From ConCert.Extraction Require Import ClosedAux.
+From Coq Require Import Arith.
+From Coq Require Import Bool.
+From Coq Require Import List.
+From Coq Require Import Psatz.
+From Coq Require Import String.
+From Equations Require Import Equations.
+From MetaCoq.Erasure Require Import EAst.
+From MetaCoq.Erasure Require Import EAstUtils.
+From MetaCoq.Erasure Require Import ECSubst.
+From MetaCoq.Erasure Require Import EInduction.
+From MetaCoq.Erasure Require Import ELiftSubst.
+From MetaCoq.Erasure Require Import EWcbvEval.
+From MetaCoq.Template Require Import utils.
+
+Import ListNotations.
+Set Equations Transparent.
+
+Notation "Σ ⊢ s ▷ t" := (eval Σ s t) (at level 50, s, t at next level) : type_scope.
+
+Derive Signature for eval.
+Derive NoConfusionHom for term.
+
+Lemma eval_tLetIn_inv Σ na val body res :
+  Σ ⊢ tLetIn na val body ▷ res ->
+  exists val_res,
+    Σ ⊢ val ▷ val_res /\
+    Σ ⊢ csubst val_res 0 body ▷ res.
+Proof.
+  intros ev.
+  depind ev; try easy.
+  - destruct args using List.rev_ind; [easy|].
+    rewrite mkApps_app in *.
+    cbn in *.
+    congruence.
+  - destruct args using List.rev_ind.
+    + cbn in *.
+      depelim H.
+      subst f.
+      now eapply IHev.
+    + rewrite mkApps_app in *.
+      cbn in *.
+      congruence.
+Qed.
+
+Inductive eval_app Σ hd arg : term -> Prop :=
+| eval_app_box argv :
+    Σ ⊢ hd ▷ tBox ->
+    Σ ⊢ arg ▷ argv ->
+    eval_app Σ hd arg tBox
+| eval_app_lambda na body argv v :
+    Σ ⊢ hd ▷ tLambda na body ->
+    Σ ⊢ arg ▷ argv ->
+    Σ ⊢ csubst argv 0 body ▷ v ->
+    eval_app Σ hd arg v
+| eval_app_ctor ind c args argv v :
+    Σ ⊢ hd ▷ mkApps (tConstruct ind c) args ->
+    Σ ⊢ arg ▷ argv ->
+    Forall value args ->
+    eval_app Σ hd arg v
+| eval_app_fix defs idx args argv v :
+    Σ ⊢ hd ▷ mkApps (tFix defs idx) args ->
+    Σ ⊢ arg ▷ argv ->
+    isStuckFix (tFix defs idx) args ->
+    Forall value args ->
+    eval_app Σ hd arg v
+| eval_app_cofix defs idx args argv v :
+    Σ ⊢ hd ▷ mkApps (tCoFix defs idx) args ->
+    Σ ⊢ arg ▷ argv ->
+    Forall value args ->
+    eval_app Σ hd arg v.
+
+Arguments isStuckFix : simpl nomatch.
+
+Lemma eval_tApp_inv Σ hd arg v :
+  Σ ⊢ tApp hd arg ▷ v ->
+  eval_app Σ hd arg v.
+Proof.
+  intros ev.
+  depind ev.
+  - now econstructor.
+  - now eapply eval_app_lambda.
+  - destruct args using List.rev_ind; [easy|].
+    clear IHargs.
+    rewrite mkApps_app in H3.
+    cbn in *.
+    apply Forall2_length in H2 as args_len.
+    rewrite !app_length in *.
+    cbn in *.
+    destruct args' as [|a' args' _] using List.rev_ind; [cbn in *; abstract lia|].
+    inversion H3; subst; clear H3.
+    assert (stuck: isStuckFix (tFix mfix idx) args').
+    { unfold isStuckFix, cunfold_fix, ETyping.unfold_fix in *.
+      destruct (nth_error mfix idx) as [f'|]; [|easy].
+      replace (rarg f') with narg by congruence.
+      unfold ETyping.is_constructor.
+      rewrite !app_length in *.
+      cbn in *.
+      rewrite (proj2 (nth_error_None _ _)) by abstract lia.
+      easy. }
+    apply (eval_app_fix Σ _ _ mfix idx args' a' _).
+    + apply eval_fix_value.
+      * easy.
+      * apply Forall2_app_r in H2.
+        easy.
+      * easy.
+    + now apply Forall2_app_r in H2.
+    + easy.
+    + apply Forall2_app_r in H2.
+      destruct H2 as (all_eval & _).
+      clear -all_eval.
+      induction all_eval; [easy|].
+      constructor; [|easy].
+      now eapply eval_to_value.
+  - destruct args as [|a args _] using List.rev_ind.
+    + cbn in *.
+      apply Forall2_length in H.
+      destruct args'; [|easy].
+      eapply IHev.
+      now f_equal.
+    + rewrite mkApps_app in H1.
+      apply Forall2_length in H as args_len.
+      rewrite !app_length in *.
+      cbn in *.
+      destruct args' as [|a' args' _] using List.rev_ind; [cbn in *; abstract lia|].
+      inversion H1; subst; clear H1.
+      assert (stuck: isStuckFix (tFix mfix idx) args').
+      { unfold isStuckFix in *.
+        destruct (ETyping.unfold_fix mfix idx) as [(? & ?)|]; [|easy].
+        unfold ETyping.is_constructor in H0.
+        destruct (Nat.ltb_spec n #|args'|).
+        - rewrite nth_error_app_lt in H0 by easy.
+          apply H0.
+        - unfold ETyping.is_constructor.
+          now rewrite (proj2 (nth_error_None _ _)) by abstract lia. }
+      apply (eval_app_fix Σ _ _ mfix idx args' a' _).
+      * apply eval_fix_value; [easy| |easy].
+        now apply Forall2_app_r in H.
+      * now apply Forall2_app_r in H.
+      * easy.
+      * apply Forall2_app_r in H.
+        destruct H as (all_eval & _).
+        clear -all_eval.
+        induction all_eval; [easy|].
+        constructor; [|easy].
+        now eapply eval_to_value.
+  - apply eval_to_value in ev1 as f'value.
+    destruct f'value.
+    + destruct t; cbn in *; try congruence.
+      * now eapply (eval_app_ctor _ _ _ _ _ []).
+      * now eapply (eval_app_cofix _ _ _ _ _ []).
+    + destruct t; cbn in *; try congruence.
+      * now econstructor.
+      * now econstructor.
+    + clear -H1 H.
+      exfalso.
+      destruct f0; try easy.
+      propify.
+      destruct H as ((_ & not_fix) & _).
+      now rewrite isFixApp_mkApps in not_fix.
+  - easy.
+Qed.
+
+Lemma eval_tApp_head Σ hd arg v :
+  Σ ⊢ tApp hd arg ▷ v ->
+  exists hdv, Σ ⊢ hd ▷ hdv.
+Proof.
+  intros ev.
+  now destruct (eval_tApp_inv _ _ _ _ ev).
+Qed.
+
+Lemma eval_tApp_arg Σ hd arg v :
+  Σ ⊢ tApp hd arg ▷ v ->
+  exists argv, Σ ⊢ arg ▷ argv.
+Proof.
+  intros ev.
+  now destruct (eval_tApp_inv _ _ _ _ ev).
+Qed.
+
+Inductive eval_spine Σ v : term -> list term -> Prop :=
+| apps_nil hd : Σ ⊢ hd ▷ v -> eval_spine Σ v hd []
+| apps_cons hd arg v :
+    eval_app Σ hd arg v ->
+    eval_spine
+    Σ ⊢ a ▷ av ->
+    app_cases
+    eval_spine Σ v (tApp hd a) (a :: args).
+
+Derive Signature for eval_spine.
+
+Lemma eval_mkApps_inv Σ hd args v :
+  Σ ⊢ mkApps hd args ▷ v ->
+  eval_spine Σ v hd args.
+Proof.
+  revert hd v.
+  induction args; intros hd v ev.
+  - now constructor.
+  - cbn in *.
+    specialize (IHargs _ _ ev).
+    depelim IHargs.
+    cbn in *.
+    destruct IHargs as (app_hdv & app_argsv & ev_app & ? & ?).
+    apply eval_tApp_inv in ev_app.
+    destruct ev_app as (hdv & argv & ev_hd & ev_arg & head_hdv).
+    exists hdv, (argv :: app_argsv).
+    split; [easy|].
+    split; [easy|].
+    easy.
+Qed.
+
+Lemma eval_mkApps_head Σ hd args v :
+  Σ ⊢ mkApps hd args ▷ v ->
+  exists hdv, Σ ⊢ hd ▷ hdv /\ (args = [] \/ head_of_app_cases hdv).
+Proof.
+  intros ev.
+  destruct (eval_mkApps_inv _ _ _ _ ev) as (? & ? & ? & ? & ?).
+  eexists.
+  easy.
+Qed.
+
+Lemma eval_mkApps_args Σ hd args v :
+  Σ ⊢ mkApps hd args ▷ v ->
+  exists argsv, Forall2 (eval Σ) args argsv.
+Proof.
+  intros ev.
+  now destruct (eval_mkApps_inv _ _ _ _ ev) as (? & ? & ?).
+Qed.
+
+Definition env_closed (Σ : EAst.global_declarations) :=
+  Forall (decl_closed ∘ snd) Σ.
+
+Lemma closed_constant Σ kn cst :
+  env_closed Σ ->
+  ETyping.declared_constant Σ kn cst ->
+  match EAst.cst_body cst with
+  | Some val => closed val = true
+  | None => True
+  end.
+Proof.
+  intros env_clos decl_const.
+  unfold ETyping.declared_constant in decl_const.
+  rewrite lookup_env_find in decl_const.
+  destruct (find _ _) eqn:find; [|easy].
+  apply find_some in find.
+  unfold env_closed in env_clos.
+  rewrite Forall_forall in env_clos.
+  specialize (env_clos _ (proj1 find)).
+  destruct p.
+  cbn in *.
+  now inversion decl_const; subst.
+Qed.
+
+Lemma eval_closed Σ t v :
+  env_closed Σ ->
+  closed t ->
+  Σ ⊢ t ▷ v ->
+  closed v.
+Proof.
+  intros env_clos clos ev.
+  induction ev using eval_evals_ind; cbn in *.
+  - easy.
+  - propify.
+    apply IHev3.
+    now apply closed_csubst.
+  - propify.
+    apply IHev2.
+    now apply closed_csubst.
+  - apply IHev.
+    pose proof (closed_constant _ _ _ env_clos H).
+    now rewrite H0 in *.
+  - propify.
+    apply IHev2.
+    unfold ETyping.iota_red.
+    apply closed_mkApps.
+    + destruct clos as (_ & clos).
+      clear -clos.
+      revert c.
+      induction brs; intros c.
+      * now rewrite nth_nth_error, nth_error_nil.
+      * cbn in *.
+        propify.
+        now destruct a, c.
+    + apply Forall_skipn.
+      eapply closed_mkApps_args.
+      apply IHev1.
+      easy.
+  - subst brs.
+    cbn in *.
+    propify.
+    apply IHev2.
+    apply closed_mkApps; [easy|].
+    clear.
+    induction n; [constructor|].
+    constructor; easy.
+  - apply IHev2.
+    specialize (IHev1 clos).
+    apply closed_mkApps_args in IHev1.
+    rewrite nth_nth_error in *.
+    destruct (nth_error _ _) eqn:nth_eq.
+    + apply nth_error_In in nth_eq.
+      now rewrite Forall_forall in IHev1.
+    + easy.
+  - easy.
+  - apply IHev2.
+    specialize (IHev1 (closed_mkApps_head _ _ clos)).
+    apply closed_mkApps.
+    + apply forallb_Forall in IHev1.
+      unfold cunfold_fix in H.
+      destruct (nth_error mfix idx) eqn:nth_eq; [|easy].
+      apply nth_error_In in nth_eq.
+      rewrite Forall_forall in IHev1.
+      exact (todo "Fixpoint unfold").
+    + exact (todo "Fixpoint args").
+  - apply closed_mkApps.
+    + cbn.
+      apply IHev.
+      now eapply closed_mkApps_head.
+    + exact (todo "Stuck fixpoint unfold").
+  - exact (todo "CoFix").
+  - exact (todo "CoFix").
+  - propify.
+    easy.
+  - easy.
+Qed.
+
+
+(*
+Ltac gen_equalities :=
+  repeat
+    match goal with
+    | [H: ?Σ ⊢ ?a ▷ ?v, IH: forall _ : term, ?Σ ⊢ ?a ▷ _ -> _ |- _ = _] =>
+      let t := constr:(IH _ H) in
+      let tty := type of t in
+      (match goal with
+       | [H: tty |- _] => fail 2
+       end || pose proof t)
+    end;
+  repeat
+    match goal with
+    | [H: ?a = ?a |- _] => clear H
+    end.
+
+Lemma eval_deterministic Σ t v v' :
+  Σ ⊢ t ▷ v ->
+  Σ ⊢ t ▷ v' ->
+  v = v'.
+Proof.
+  intros ev1.
+  revert v'.
+  induction ev1 using eval_evals_ind; intros v' ev2.
+  - admit.
+  - apply eval_tApp_inv in ev2.
+    destruct ev2 as (hdv & argv & ev_hd & ev_arg & hd_app).
+    inversion hd_app; subst; clear hd_app;
+      gen_equalities; try congruence; try solve_discr.
+    inversion H2; subst.
+    admit.
+  - apply eval_tLetIn in ev2.
+    destruct ev2 as (? & ? & ?).
+    gen_equalities.
+    subst.
+    now gen_equalities.
+  - depind ev2.
+    + destruct args using List.rev_ind; [easy|].
+      now rewrite mkApps_app in H5.
+    + destruct args using List.rev_ind; [|now rewrite mkApps_app in *].
+      cbn in *.
+      subst f.
+      apply Forall2_length in H.
+      destruct args'; [|easy].
+      cbn in *.
+      eapply IHev2; easy.
+    + unfold ETyping.declared_constant in *.
+      replace body0 with body in * by congruence.
+      now gen_equalities.
+    + easy.
+  - depind ev2.
+    + gen_equalities.
+      solve_discr.
+      inversion H; subst; clear H.
+      now gen_equalities.
+    + gen_equalities.
+      solve_discr.
+    + destruct args using List.rev_ind; [easy|].
+      rewrite mkApps_app in H3.
+      solve_discr.
+    + destruct args using List.rev_ind; cycle 1.
+      { now rewrite mkApps_app in H1. }
+      cbn in *.
+      subst f.
+      apply Forall2_length in H.
+      destruct args'; [|easy].
+      cbn in *.
+      easy.
+    + admit.
+    + easy.
+  - depind ev2; subst.
+    + gen_equalities.
+      solve_discr.
+    + inversion H; subst.
+      now gen_equalities.
+    + destruct args using List.rev_ind; [easy|].
+      now rewrite mkApps_app in *.
+    + destruct args using List.rev_ind; cycle 1.
+      { now rewrite mkApps_app in H1. }
+      cbn in *.
+      subst f.
+      apply Forall2_length in H.
+      destruct args'; [|easy].
+      easy.
+    + apply eval_mkApps_inv in ev1_1.
+      destruct ev1_1 as (hdv & argsv & ev_hd & ev_args & disc).
+      destruct disc as [->|].
+      * cbn in *.
+        gen_equalities.
+        subst.
+        assert (Σ ⊢ tCoFix mfix idx ▷ tCoFix mfix idx); [|gen_equalities; easy].
+        now apply eval_atom.
+      * admit.
+    + easy.
+  - admit.
+  - admit.
+  - admit.
+  - admit.
+  - admit.
+    assert (Σ ⊢ tProj (i, pars, arg) discr ▷ tBox).
+    { now apply eval_proj_box. }
+    gen_equalities.
+      eapply IHev2
+      subst brs.
+      cbn in *.
+      easy.
+      apply IHev1.
+      subst f.
+      2: {
+      gen_equalities; try congruence; try solve_discr.
+
+    +
+    + gen_equalities; congruence.
+    + gen_equalities; subst.
+      inversion H2; subst.
+      gen_equalities.
+      admit.
+    + gen_equalities.
+      solve_discr.
+    + gen_equalities.
+      solve_discr.
+    + gen_equai
+    depelim ev2.
+    + gen_equalities; congruence.
+    + gen_equalities.
+      inversion H2.
+      subst.
+      now gen_equalities.
+    + destruct args as [|a'' args _] using List.rev_ind; [easy|].
+      rewrite mkApps_app in H3.
+      cbn in *.
+      inversion H3; subst; clear H3.
+
+      replace f with (mkApps f0 args) in * by congruence.
+      apply eval_mkApps_inv in ev2_2.
+      destruct ev2_2 as (? & ? & ? & ? & ?).
+
+      gen_equalities.
+      subst a'0.
+      inversion H2; subst; clear H2.
+      apply IHev1_3.
+      let x := (has_hypothesis_of_type term) in
+      match x with
+      | 0 => idtac "foo"
+      | 1 => idtac "bar"
+      end.
+      gen_equalities.
+      gen_equalities.
+    +
+    apply eval_tApp_inv in ev2 as (hdv & argv & ev_hd & ev_arg & hd_cases).
+    apply IHev1_3.
+    depelim hd_cases; try solve_congr.
+    + apply IHev1_3.
+    +
+    inversion hd_cases; subst.
+    apply eval_tApp_head in ev2.
+    destruct ev2 as (hdv & ev_hd & hdv_cases).
+    depelim hdv_cases;
+      specialize (IHev1_1 _ ev_hd); try congruence.
+*)
+
+(*
+Lemma eval_tLambda_to_tBox Σ na body :
+  Σ ⊢ tLambda na body ▷ tBox ->
+  False.
+Proof.
+  intros.
+  depelim H.
+  - destruct args using List.rev_ind; [easy|now rewrite mkApps_app in *].
+  - destruct args' using List.rev_ind; [easy|now rewrite mkApps_app in *].
+Qed.
+
+Lemma eval_tApp_tLambda Σ na body hd v :
+  Σ ⊢ tApp (tLambda na body) hd ▷ v ->
+  Σ ⊢ csubst hd 0 body ▷ v.
+Proof.
+  intros.
+  depelim H.
+  - now apply eval_tLambda_to_tBox in H.
+  - easy.
+*)
